lockserver/server.dfy
@@ -1,21 +1,92 @@
 include "types.dfy"
+include "network.dfy"
 
 module Server {
 import opened Types
+import opened Network
 
+datatype ResourceStatus = Free | Held(client:Id)
 
 datatype Server = Server(
     id:Id,                  
-    resource_available:bool,    // is this server free to grant requests?
+    resource:ResourceStatus,    // is this server free to grant requests?
     epoch_map:map<Id, Epoch>    // maps each client to the latest epoch seen from that client
 )
 
+/* Server initial state */
 predicate ServerInit(s:Server, id:Id) {
     && s.id == id
-    && s.resource_available
+    && s.resource.Free?
     && s.epoch_map == map[]
 }
 
+/* Server next state */
+predicate ServerNext(s:Server, s':Server, recvIo:IoOpt, sendIo:IoOpt) 
+{
+    && recvIo.Some? 
+    && s'.id == s.id
+    && match recvIo.p.msg {
+        case Request(e) => ProcessRequest(s, s', recvIo, sendIo)
+        case Release(e) => ProcessRelease(s, s', recvIo, sendIo)
+        case _ => ServerStutter(s, s', sendIo)
+    }
+}
 
+/* Server processing a Request message from a client */
+predicate ProcessRequest(s:Server, s':Server, recvIo:IoOpt, sendIo:IoOpt) 
+    requires recvIo.Some? && recvIo.p.msg.Request?
+{
+    var e := recvIo.p.msg.e;
+    if !s.resource.Free? then
+        ProcessRequest_Reject(s, s', recvIo.p, sendIo)
+    else if e > s.epoch_map[recvIo.p.src] then
+        ProcessRequest_Grant(s, s', recvIo.p, sendIo)
+    else 
+        ProcessRequest_Reject(s, s', recvIo.p, sendIo)
+}
 
+predicate ProcessRequest_Grant(s:Server, s':Server, p:Packet, sendIo:IoOpt) 
+    requires p.msg.Request?
+    requires p.msg.e > s.epoch_map[p.src]
+{
+    && s'.epoch_map == s.epoch_map[p.src := p.msg.e]
+    && s'.resource == Held(p.src)
+    && sendIo == Some(Packet(s.id, p.src, Grant(p.msg.e)))
+}
+
+predicate ProcessRequest_Reject(s:Server, s':Server, p:Packet, sendIo:IoOpt) 
+    requires p.msg.Request?
+{
+    && s'.epoch_map == s.epoch_map
+    && s'.resource == s.resource
+    && sendIo == Some(Packet(s.id, p.src, Reject(p.msg.e)))
+}
+
+/* Server processing a Release message from a client */
+predicate ProcessRelease(s:Server, s':Server, recvIo:IoOpt, sendIo:IoOpt) 
+    requires recvIo.Some? && recvIo.p.msg.Release?
+{
+    var e := recvIo.p.msg.e;
+    if s.resource.Free? then 
+        ServerStutter(s, s', sendIo)
+    else if 
+        && s.resource.client == recvIo.p.src 
+        && recvIo.p.src in s.epoch_map
+        && s.epoch_map[recvIo.p.src] == e then
+        ProcessRelease_Release(s, s, sendIo)
+    else
+        ServerStutter(s, s', sendIo)
+}
+
+predicate ProcessRelease_Release(s:Server, s':Server, sendIo:IoOpt) {
+    && s'.epoch_map == s.epoch_map
+    && s'.resource == Free
+    && sendIo == None
+}
+
+/* Server taking a stutter step */
+predicate ServerStutter(s:Server, s':Server, sendIo:IoOpt) {
+    && s' == s
+    && sendIo == None
+}
 }
